sandbox/Compile.v
@@ -1,0 +1,46 @@
+Require Import Codes.
+Require Import Combinators.
+Require Import DeBruijn.
+Require Import BohmTrees.
+
+Fixpoint compile {Var : Set} (t : Term Var) : Code Var :=
+  match t with
+  | TOP%term => TOP%code
+  | BOT%term => BOT%code
+  | x || y => (compile x || compile y)%code
+  | x (+) y => (compile x (+) compile y)%code
+  | x * y => (compile x * compile y)%code
+  | term_var v => code_var v
+  | term_lambda x => code_abs id (compile x)
+  end.
+
+(* TODO this needs to be changed to get [decompile_compile] to hold *)
+Fixpoint decompile {Var : Set} (c : Code Var) : Term Var :=
+  match c with
+  | TOP%code => TOP
+  | BOT%code => BOT
+  | I => DeBruijn.I
+  | K => DeBruijn.K
+  | B => DeBruijn.B
+  | C => DeBruijn.C
+  | S => DeBruijn.S
+  | J => (DeBruijn.I || DeBruijn.I)
+  | R => (DeBruijn.I || DeBruijn.I)
+  | (x || y)%code => (decompile x || decompile y)
+  | (x (+) y)%code => (decompile x (+) decompile y)
+  | (x * y)%code => (decompile x * decompile y)
+  | code_var v => term_var v
+  end.
+
+(* maybe restrict [t] to Bohm trees *)
+Lemma decompile_compile (Var : Set) (t : Term Var) : decompile (compile t) = t.
+Proof.
+  induction t; simpl; auto.
+  - rewrite IHt1, IHt2; reflexivity.
+  - rewrite IHt1, IHt2; reflexivity.
+  - rewrite IHt1, IHt2; clear IHt1 IHt2.
+    case_eq t1; auto.
+    + admit. (* easy *)
+    + admit. (* easy *)
+  - admit. (* TODO this is the crucial case *)
+Qed.
